# Distribuição de Hotelling

Sejam $Z \sim N_p(\boldsymbol{0}, I)$ e [$M \sim \mathrm{Wishart}_p(I,m)$](wishart.qmd)
independentes. Dizemos que
$$
H = m \cdot Z^T M^{-1} Z
$$

tem distribuição $T^2$ de Hotelling.

::: {.callout-note, title="Notação"}
$$
H \sim T^2(p,m)
$$
:::

*Teorema 1.*

Se $\boldsymbol{X}_n \sim N_p(\boldsymbol{\mu}, \Sigma)$ e $M \sim
\mathrm{Wishart}_p(\Sigma, m)$, então

$$
m \cdot (\boldsymbol{X} - \mu)^T M^{-1} (\boldsymbol{X} - \mu) \sim T^2(p,m)
$$

*Prova*.

Note que

$$
Z = \Sigma^{-1/2}(\boldsymbol{X} - \boldsymbol{\mu}) \sim N_p(0, I)
$$

e
$$
M^*= \Sigma^{-1/2}M \Sigma^{-1/2} \sim \mathrm{Wishart}_p(I, m),\ \text{pois}
\Sigma^{-1/2}M\Sigma^{-1/2} = I
$$

Por definição,

$$
m Z^t M^* Z = m(\boldsymbol{X} - \boldsymbol{\mu})^T M^{-1} (\boldsymbol{X} -
\boldsymbol{\mu}) \sim T^2(p,m)
$$
